working version of custom types w/o params

experiments/CustomTypes.v
@@ -2,45 +2,34 @@ Require Import List.
 Import ListNotations.
 
 Require Import Common HList.
-Require Vector.
+Require Vector Fin.
+
+Global Arguments Vector.nil {_}.
+Global Arguments Vector.cons {_} _ {_} _.
 
 Set Implicit Arguments.
 Set Maximal Implicit Insertion.
 
-Fixpoint varargs (n_args : nat) : Type :=
-  match n_args with
-  | 0 => Type
-  | S n_args => Type -> varargs n_args
+Inductive type (kind_ctx : nat) : Type :=
+| Arrow : type kind_ctx -> type kind_ctx -> type kind_ctx
+| Base : Fin.t kind_ctx -> type kind_ctx
+.
+
+Definition type_eq_dec kind_ctx (ty1 ty2 : type kind_ctx) : {ty1 = ty2} + {ty1 <> ty2}.
+  decide equality.
+  auto using Fin.eq_dec.
+Defined.
+
+Fixpoint type_denote {kind_ctx} (v : Vector.t Type kind_ctx) (ty : type kind_ctx) : Type :=
+  match ty with
+  | Arrow ty1 ty2 => type_denote v ty1 -> type_denote v ty2
+  | Base m => Vector.nth v m
   end.
 
-Inductive type (kind_ctx : list nat) : Type :=
-| Arrow : type kind_ctx -> type kind_ctx -> type kind_ctx
-| Base : forall n, member n kind_ctx -> Vector.t (type kind_ctx) n -> type kind_ctx
-.
-(* feeling lazy... *)
-Axiom type_eq_dec : forall kind_ctx (ty1 ty2 : type kind_ctx), {ty1 = ty2} + {ty1 <> ty2}.
-
-Fixpoint varapply {n} (f : varargs n) (args : Vector.t Type n) : Type :=
-  match args in Vector.t _ n0 return varargs n0 -> Type with
-  | Vector.nil => fun f => f
-  | Vector.cons ty v => fun f => varapply (f ty) v
-  end f.
-
-Fixpoint type_denote {kind_ctx} (h : hlist varargs kind_ctx) (ty : type kind_ctx) : Type :=
-  let fix go_vec {n} (v : Vector.t (type kind_ctx) n) : Vector.t Type n :=
-      match v with
-      | Vector.nil => Vector.nil
-      | Vector.cons ty v => Vector.cons (type_denote h ty) (go_vec v)
-      end
-  in match ty with
-     | Arrow ty1 ty2 => type_denote h ty1 -> type_denote h ty2
-     | Base m args => varapply (hget h m) (go_vec args)
-     end.
-
-Fixpoint insert_recursive_calls {kind_ctx} (l : list (type kind_ctx)) (rec_ty : type kind_ctx) (motive_ty : type kind_ctx) : list (type kind_ctx) :=
+Fixpoint insert_recursive_calls {kind_ctx} (l : list (type kind_ctx)) (rec_ty : Fin.t kind_ctx) (motive_ty : type kind_ctx) : list (type kind_ctx) :=
   match l with
   | [] => []
-  | ty :: l => (if type_eq_dec ty rec_ty
+  | ty :: l => (if type_eq_dec ty (Base rec_ty)
               then [ty;  motive_ty]
               else []) ++ insert_recursive_calls l rec_ty motive_ty
   end.
@@ -51,38 +40,191 @@ Fixpoint varargs_type {kind_ctx} (l : list (type kind_ctx)) (R : type kind_ctx) 
   | ty :: l => Arrow ty (varargs_type l R)
   end.
 
-Definition case_types {kind_ctx} (l : list (list (type kind_ctx))) (rec_ty motive_ty : type kind_ctx)
+Definition case_types {kind_ctx} (l : list (list (type kind_ctx))) (rec_ty : Fin.t kind_ctx) (motive_ty : type kind_ctx)
     : list (type kind_ctx) :=
   List.map (fun l => varargs_type (insert_recursive_calls l rec_ty motive_ty) motive_ty) l.
 
-Module type_context.
-  Inductive t : list nat -> Type :=
-  | nil : t []
-  | cons kind_ctx n_params
-         (denotation : varargs n_params)
-         (constrs : list (list (type kind_ctx)))
-
-    :
-      t kind_ctx -> t (n_params :: kind_ctx)
-  .
-End type_context.
-
-Inductive expr {kind_ctx} (ty_ctx : type_context.t kind_ctx)
+Inductive expr {kind_ctx} (constr_ctx : Vector.t (list (list (type kind_ctx))) kind_ctx)
   : list (type kind_ctx) -> type kind_ctx -> Type :=
-| Var : forall {ty l}, member ty l -> expr ty_ctx l ty
-| Lam : forall {ty1 ty2 l}, expr ty_ctx (ty1 :: l) ty2 -> expr ty_ctx l (Arrow ty1 ty2)
-| App : forall {ty1 ty2 l}, expr ty_ctx l (Arrow ty1 ty2) -> expr ty_ctx l ty1 -> expr ty_ctx l ty2
-| Constr : forall n (m : member n kind_ctx) (actual_type_params : Vector.t (type kind_ctx) n) arg_tys l,
-    member arg_tys (hget constr_env m) ->
-    hlist (expr ty_ctx l) arg_tys -> expr ty_ctx l (Base m actual_type_params)
-| Elim : forall n (m : member n kind_ctx) (actual_type_params : Vector.t (type kind_ctx) n) motive_ty l,
-    let target_ty := Base m actual_type_params in
-    hlist (expr ty_ctx l) (case_types (hget constr_env m) target_ty motive_ty) ->
-    expr ty_ctx l target_ty ->
-    expr ty_ctx l motive_ty
+| Var : forall {ty l},
+    member ty l ->
+    expr constr_ctx l ty
+| Lam : forall {ty1 ty2 l},
+    expr constr_ctx (ty1 :: l) ty2 ->
+    expr constr_ctx l (Arrow ty1 ty2)
+| App : forall {ty1 ty2 l},
+    expr constr_ctx l (Arrow ty1 ty2) ->
+    expr constr_ctx l ty1 ->
+    expr constr_ctx l ty2
+| Constr : forall (x : Fin.t kind_ctx) arg_tys l,
+    member arg_tys (Vector.nth constr_ctx x) ->
+    hlist (expr constr_ctx l) arg_tys ->
+    expr constr_ctx l (Base x)
+| Elim : forall (x : Fin.t kind_ctx) motive_ty l,
+    hlist (expr constr_ctx l) (case_types (Vector.nth constr_ctx x) x motive_ty) ->
+    expr constr_ctx l (Base x) ->
+    expr constr_ctx l motive_ty
 .
+Arguments Var {_ _ _ _} _.
+Arguments Elim {_ _} _ _ {_} _ _.
 
-Fixpoint expr_denote {kind_ctx c_env l} {ty : type kind_ctx} (e : expr l ty)
-  : forall (ty_sub : hlist varargs kind_ctx)
-      (c_sub :
-type_denote :=
+Fixpoint varargs_type_denote_apply {kind_ctx}
+  (ty_sub : Vector.t Type kind_ctx)
+  {l R} : forall (f : type_denote ty_sub (varargs_type l R))
+            (args : hlist (type_denote ty_sub) l), type_denote ty_sub R :=
+  match l as l0 with
+  | [] => fun f _ => f
+  | ty :: l => fun f args => varargs_type_denote_apply _ (f (hhead args)) (htail args)
+  end.
+
+Definition expr_denote {kind_ctx constr_ctx}
+         (ty_sub : Vector.t Type kind_ctx)
+         (c_sub : forall (x : Fin.t kind_ctx),
+             forall arg_tys (m : member arg_tys (Vector.nth constr_ctx x)),
+               type_denote ty_sub (varargs_type arg_tys (Base x)))
+         (e_sub : forall (x : Fin.t kind_ctx) motive_ty,
+               type_denote ty_sub
+                    (varargs_type (case_types (Vector.nth constr_ctx x) x motive_ty)
+                                  (Arrow (Base x) motive_ty)))
+         {l} {ty : type kind_ctx} (e : expr constr_ctx l ty)
+  (env : hlist (type_denote ty_sub) l) : type_denote ty_sub ty.
+  refine (
+      let fix go {l} {ty : type kind_ctx} (e : expr constr_ctx l ty)
+                (env : hlist (type_denote ty_sub) l) : type_denote ty_sub ty :=
+          let fix go_hlist {l} {tys : list (type kind_ctx)} (h : hlist (expr constr_ctx l) tys)
+                  (env : hlist (type_denote ty_sub) l) : hlist (type_denote ty_sub) tys :=
+              match h with
+              | hnil => hnil
+              | hcons e h => hcons (go e env) (go_hlist h env)
+              end
+          in
+          match e in expr _ l0 ty0
+          return hlist (type_denote ty_sub) l0 -> type_denote ty_sub ty0
+          with
+          | Var m => fun h => hget h m
+          | Lam e => fun h x => go e (hcons x h)
+          | App e1 e2 => fun h => go e1 h (go e2 h)
+          | Constr x m args => fun h =>
+              varargs_type_denote_apply ty_sub (c_sub x _ m) (go_hlist args h)
+          | Elim x motive_ty cases target => fun h =>
+              varargs_type_denote_apply ty_sub (e_sub x motive_ty) (go_hlist cases h) (go target h)
+          end env
+      in go e env
+    ).
+Defined.
+
+(* The stdlib notations for vector are broken so we roll our own. *sigh* *)
+Delimit Scope vector_scope with vector.
+Bind Scope vector_scope with Vector.t.
+
+Notation "[ ]" := Vector.nil : vector_scope.
+Notation "h :: t" := (Vector.cons h t) (at level 60, right associativity) : vector_scope.
+Notation "[ x ]" := (x :: [])%vector : vector_scope.
+Notation "[ x ; y ; .. ; z ]" := (x :: (y :: .. (z :: []) ..))%vector : vector_scope.
+
+Delimit Scope hlist_scope with hlist.
+Bind Scope hlist_scope with hlist.
+
+Notation "[ ]" := hnil : hlist_scope.
+Notation "h :: t" := (hcons h t) (at level 60, right associativity) : hlist_scope.
+Notation "[ x ]" := (x :: [])%hlist : hlist_scope.
+Notation "[ x ; y ; .. ; z ]" := (x :: (y :: .. (z :: []) ..))%hlist : hlist_scope.
+
+Module examples.
+  Definition kind_ctx := 2.
+
+  Module bool.
+    Definition index : Fin.t kind_ctx := Fin.F1.
+    Definition ty : type kind_ctx := Base index.
+    Definition denotation : Type := Datatypes.bool.
+    Definition constrs : list (list (type kind_ctx)) := [[]; []].
+
+    Definition true : member [] constrs := Here.
+    Definition false : member [] constrs := There Here.
+  End bool.
+
+  Module nat.
+    Definition index : Fin.t kind_ctx := Fin.FS Fin.F1.
+    Definition ty : type kind_ctx := Base index.
+    Definition denotation : Type := Datatypes.nat.
+    Definition constrs : list (list (type kind_ctx)) := [[]; [ty]].
+
+    Definition O : member [] constrs := Here.
+    Definition S : member [ty] constrs := There Here.
+  End nat.
+
+  Definition constr_ctx : Vector.t (list (list (type kind_ctx))) kind_ctx :=
+    [bool.constrs; nat.constrs].
+
+  Definition ty_sub : Vector.t Type kind_ctx :=
+    [bool.denotation; nat.denotation].
+
+  Ltac invc_member :=
+    repeat match goal with
+    | [ H : member _ _ |- _ ] => invc H
+    end.
+
+  Ltac destruct_fin :=
+    match goal with
+    | [ x : Fin.t _ |- _ ] =>
+      (destruct x using Fin.caseS'; [|destruct_fin]) || destruct x using Fin.case0
+    end.
+
+  Definition c_sub
+             (x : Fin.t kind_ctx)
+             arg_tys
+             (m : member arg_tys (Vector.nth constr_ctx x))
+    : type_denote ty_sub (varargs_type arg_tys (Base x)).
+    destruct_fin.
+    - invc_member.
+      + exact true.
+      + exact false.
+    - invc_member.
+      + exact O.
+      + exact S.
+  Defined.
+
+  Definition e_sub
+             (x : Fin.t kind_ctx)
+             motive_ty
+    : type_denote ty_sub (varargs_type (case_types (Vector.nth constr_ctx x) x motive_ty)
+                                  (Arrow (Base x) motive_ty)).
+    destruct_fin.
+    - exact (bool_rect _).
+    - exact (nat_rect _).
+  Defined.
+
+
+  Module programs.
+    Definition andb {l} : expr constr_ctx l (Arrow bool.ty (Arrow bool.ty bool.ty)).
+      refine (Lam (Lam (Elim bool.index _ _ (Var (There Here))))).
+      exact [Var Here; Constr(constr_ctx := constr_ctx) bool.index bool.false []]%hlist.
+    Defined.
+
+    Definition add {l} : expr constr_ctx l (Arrow nat.ty (Arrow nat.ty nat.ty)).
+      refine (Lam (Elim nat.index _ _ (Var Here))).
+refine [Lam (Var Here);
+             Lam (Lam (Lam (Constr(constr_ctx := constr_ctx) nat.index nat.S [App (Var (There Here)) (Var Here)])))]%hlist.
+    Defined.
+  End programs.
+
+  Eval compute in expr_denote ty_sub c_sub e_sub programs.andb hnil.
+  Check eq_refl : expr_denote ty_sub c_sub e_sub programs.andb hnil = andb.
+
+  Definition add a b :=
+    @nat_rect (fun _ => nat -> nat)     (* this is `add` *)
+              (fun b => b)
+              (fun a IHa b => S (IHa b))
+              a b.
+
+  Example add_Nat_add : forall m n, add m n = Nat.add m n.
+  Proof.
+    induction m; simpl; intros.
+    - reflexivity.
+    - now rewrite IHm, plus_n_Sm.
+  Qed.
+
+  Eval compute in expr_denote ty_sub c_sub e_sub programs.add hnil.
+  Eval compute in add.
+  Check eq_refl : expr_denote ty_sub c_sub e_sub programs.add hnil = add.
+End examples.
